addBefore and addAfter as linked lists

project.dfy
@@ -1,89 +1,100 @@
+/**
+    om - Order Maintained
+    ds - Data Structure
+ */
 module Collections {
     
     class Node {
         var omLabel: int;
         var omValue: int;
 
-        constructor (omLbl: int, omVal: int)
+        var previous: Node?;
+        var next: Node?;
+
+        var index: int;
+
+        constructor (omLbl: int, omVal: int, idx: int)
+            ensures omLabel == omLbl && omValue == omVal && index == idx
         {
             new;
             omLabel := omLbl;
             omValue := omVal;
+
+            index := idx;
         }
     }
 
-    trait OMDataStructTrait
-    {
+    trait OMDataStructTrait {
         var maxCapacity: int;
-        var omDS: array<Node?>;
+        var omDS: Node?;
 
-        ghost var omDsSeq: seq<Node?>;
+        ghost var omDsSeq: seq<Node>;
 
-        method addBefore(x: int, y: int)
+        method addBefore(x: int, yNode: Node)
             // Check y exists in DS
-            requires exists i :: 0 <= i < |omDsSeq| && omDsSeq[i] != null && omDsSeq[i].omValue == y
+            requires exists i :: 0 <= i < |omDsSeq| && omDsSeq[i].omValue == yNode.omValue
             // Check x doesn't exist in DS
-            requires forall i :: 0 <= i < |omDsSeq| && omDsSeq[i] != null && omDsSeq[i].omValue != x
+            requires forall i :: 0 <= i < |omDsSeq| && omDsSeq[i].omValue != x
             // Check x's position is less than y's position
-            ensures exists i,j :: 0 <= i < j < |omDsSeq| && (omDsSeq[i] != null && omDsSeq[i].omValue == x) && (omDsSeq[j] != null && omDsSeq[j].omValue == y)
-            modifies omDsSeq
+            ensures exists i,j :: 0 <= i < j < |omDsSeq| && omDsSeq[i].omValue == x && omDsSeq[j].omValue == yNode.omValue
+            modifies yNode, yNode.previous, omDS, omDsSeq
 
-        method addAfter(x: int, y: int)
+        method addAfter(x: int, yNode: Node)
             // Check y exists in DS
-            requires exists i :: 0 <= i < |omDsSeq| && omDsSeq[i] != null && omDsSeq[i].omValue == y
+            requires exists i :: 0 <= i < |omDsSeq| && omDsSeq[i].omValue == yNode.omValue
             // Check x doesn't exist in DS
-            requires forall i :: 0 <= i < |omDsSeq| && omDsSeq[i] != null && omDsSeq[i].omValue != x
+            requires forall i :: 0 <= i < |omDsSeq| && omDsSeq[i].omValue != x
             // Check x's position is greater than y's position
-            ensures exists i,j :: 0 <= i < j < |omDsSeq| && (omDsSeq[i] != null && omDsSeq[i].omValue == y) && (omDsSeq[j] != null && omDsSeq[j].omValue == x)
-            modifies omDsSeq
+            ensures exists i,j :: 0 <= i < j < |omDsSeq| && omDsSeq[i].omValue == yNode.omValue && omDsSeq[j].omValue == x
+            modifies omDS, omDsSeq, yNode, yNode.next
 
-        method add(x: int)
-            // Check x doesn't exist in DS
-            requires forall i :: 0 <= i < |omDsSeq| && omDsSeq[i] != null && omDsSeq[i].omValue != x
-            // Check x exists random position in DS
-            ensures exists i :: 0 <= i < |omDsSeq| && omDsSeq[i] != null && omDsSeq[i].omValue == x
-            modifies omDsSeq
+        // method add(x: int)
+        //     // Check x doesn't exist in DS
+        //     requires forall i :: 0 <= i < |omDsSeq| && omDsSeq[i] != null && omDsSeq[i].omValue != x
+        //     // Check x exists random position in DS
+        //     ensures exists i :: 0 <= i < |omDsSeq| && omDsSeq[i] != null && omDsSeq[i].omValue == x
+        //     modifies omDsSeq
 
-        method element(x: int) returns (exist: bool)
-            // At some position, if x exists then return true otherwise false
-            ensures exist == false || ((exists i :: 0 <= i < |omDsSeq| && (omDsSeq[i] != null && omDsSeq[i].omValue == x)) && exist == true)
+        // method element(x: int) returns (exist: bool)
+        //     // At some position, if x exists then return true otherwise false
+        //     ensures exist == false || ((exists i :: 0 <= i < |omDsSeq| && (omDsSeq[i] != null && omDsSeq[i].omValue == x)) && exist == true)
 
-        method before(x: int, y: int) returns (isBefore: bool)
-            // Checks x and y are different values
-            requires x != y
-            // Check x exists in DS
-            requires exists i :: 0 <= i < |omDsSeq| && omDsSeq[i] != null && omDsSeq[i].omValue == x
-            // Check y exists in DS
-            requires exists j :: 0 <= j < |omDsSeq| && omDsSeq[j] != null && omDsSeq[j].omValue == y
-            // If x's position is less than y's position then return true otherwise false
-            ensures exists i,j :: 0 <= i < j < |omDsSeq| && ((((omDsSeq[i] != null && omDsSeq[i].omValue == x) && (omDsSeq[j] != null && omDsSeq[j].omValue == y)) && isBefore == true) || isBefore == false)
+        // method before(x: int, y: int) returns (isBefore: bool)
+        //     // Checks x and y are different values
+        //     requires x != y
+        //     // Check x exists in DS
+        //     requires exists i :: 0 <= i < |omDsSeq| && omDsSeq[i] != null && omDsSeq[i].omValue == x
+        //     // Check y exists in DS
+        //     requires exists j :: 0 <= j < |omDsSeq| && omDsSeq[j] != null && omDsSeq[j].omValue == y
+        //     // If x's position is less than y's position then return true otherwise false
+        //     ensures exists i,j :: 0 <= i < j < |omDsSeq| && ((((omDsSeq[i] != null && omDsSeq[i].omValue == x) && (omDsSeq[j] != null && omDsSeq[j].omValue == y)) && isBefore == true) || isBefore == false)
 
-        method append(x: int)
-            // Check x doesn't exist in DS
-            requires forall i :: 0 <= i < |omDsSeq| && (omDsSeq[i] != null && omDsSeq[i].omValue != x)
-            // If DS size is 1 then x is at the start of DS or DS size is greater than 1 then x is at the end of the DS.
-            ensures ((|omDsSeq| == 1 && (omDsSeq[0] != null && omDsSeq[0].omValue == x)) || (|omDsSeq| > 1 && (exists i :: 0 <= i < |omDsSeq|-1 && ((omDsSeq[i] != null && omDsSeq[i+1] == null) && omDsSeq[i].omValue == x))))
-            modifies omDsSeq
+        // method append(x: int)
+        //     // Check x doesn't exist in DS
+        //     requires forall i :: 0 <= i < |omDsSeq| && (omDsSeq[i] != null && omDsSeq[i].omValue != x)
+        //     // If DS size is 1 then x is at the start of DS or DS size is greater than 1 then x is at the end of the DS.
+        //     ensures ((|omDsSeq| == 1 && (omDsSeq[0] != null && omDsSeq[0].omValue == x)) || (|omDsSeq| > 1 && (exists i :: 0 <= i < |omDsSeq|-1 && ((omDsSeq[i] != null && omDsSeq[i+1] == null) && omDsSeq[i].omValue == x))))
+        //     modifies omDsSeq
 
-        method prepend(x: int)
-            // At least 1 position should be empty
-            requires exists i :: 0 <= i < |omDsSeq| && omDsSeq[i] == null
-            // Last element should be null
-            requires |omDsSeq| > 0 && omDsSeq[|omDsSeq|-1] == null
-            // Check x doesn't exist in DS
-            requires forall i :: 0 <= i < |omDsSeq| && omDsSeq[i] != null && omDsSeq[i].omValue != x
-            // Check x is at the start of the DS always
-            ensures |omDsSeq| > 0 && omDsSeq[0] != null && omDsSeq[0].omValue == x
-            modifies omDsSeq
+        // method prepend(x: int)
+        //     // At least 1 position should be empty
+        //     requires exists i :: 0 <= i < |omDsSeq| && omDsSeq[i] == null
+        //     // Last element should be null
+        //     requires |omDsSeq| > 0 && omDsSeq[|omDsSeq|-1] == null
+        //     // Check x doesn't exist in DS
+        //     requires forall i :: 0 <= i < |omDsSeq| && omDsSeq[i] != null && omDsSeq[i].omValue != x
+        //     // Check x is at the start of the DS always
+        //     ensures |omDsSeq| > 0 && omDsSeq[0] != null && omDsSeq[0].omValue == x
+        //     modifies omDsSeq
 
-        method remove(x: int)
-            // Check x exists in DS
-            requires exists i :: 0 <= i < |omDsSeq| && omDsSeq[i] != null && omDsSeq[i].omValue == x
-            // Check each value is unique
-            requires forall i :: 0 <= i < |omDsSeq|-1 && omDsSeq[i] != null && (forall j :: i < j < |omDsSeq| && omDsSeq[j] != null && omDsSeq[i].omValue != omDsSeq[j].omValue)
-            // Check x doesn't exist in DS
-            ensures forall i :: 0 <= i < |omDsSeq| && ((omDsSeq[i] != null && omDsSeq[i].omValue != x) || omDsSeq[i] == null)
-            modifies omDsSeq
+        // method remove(x: int)
+        //     // Check x exists in DS
+        //     requires exists i :: 0 <= i < |omDsSeq| && omDsSeq[i] != null && omDsSeq[i].omValue == x
+        //     // Check each value is unique
+        //     requires forall i :: 0 <= i < |omDsSeq|-1 && omDsSeq[i] != null && (forall j :: i < j < |omDsSeq| && omDsSeq[j] != null && omDsSeq[i].omValue != omDsSeq[j].omValue)
+        //     // Check x doesn't exist in DS
+        //     ensures forall i :: 0 <= i < |omDsSeq| && ((omDsSeq[i] != null && omDsSeq[i].omValue != x) || omDsSeq[i] == null)
+        //     modifies omDsSeq
     }
 
     class OMDataStruct extends OMDataStructTrait {
@@ -104,357 +115,276 @@ module Collections {
             // Insert before 0 triggers relabeling. Thus, not covered in initial version.
             // [0, 4, 8, 12] - labels
             // [11, 46, 30, 4] - values
-            var node0 := new Node(0, 11);
-            var node1 := new Node(4, 46);
-            var node2 := new Node(8, 30);
-            var node3 := new Node(12, 4);
+            var node0 := new Node(0, 11, 0);
+            var node1 := new Node(4, 46, 1);
+            var node2 := new Node(8, 30, 2);
+            var node3 := new Node(12, 4, 3);
 
-            omDS := new Node?[maxCapacity];
-            omDS[0] := node0;
-            omDS[1] := node1;
-            omDS[2] := node2;
-            omDS[3] := node3;
+            omDS := node0;
+            node0.next := node1;
+            node1.next := node2;
+            node2.next := node3;
+            node3.next := null;
 
-            omDsSeq := computeOmDsSeq(omDS, omDS.Length-1);
+            node3.previous := node2;
+            node2.previous := node1;
+            node1.previous := node0;
+            node0.previous := null;
+
+            omDsSeq := [node0, node1, node2, node3];
         }
 
-        function computeOmDsSeq(omDS: array<Node?>, index: nat): seq<Node?>
-            requires 0 <= index < omDS.Length
-            reads omDS
-        {
-            if index == 0 then [omDS[0]] else computeOmDsSeq(omDS, index-1) + [omDS[index]]
-        }
-
-        // Will be used till a memory pointer manupulation way is found.
-        method findIndex(x: int) returns (index: int)
-            // Check y exists in the array
-            requires exists i :: 0 <= i < omDS.Length && omDS[i] != null && omDS[i].omValue == x
-            ensures 0 <= index < omDS.Length
-            ensures omDS[index] != null && omDS[index].omValue == x
-        {
-            index := 0;
-            while(index < omDS.Length)
-                // Swapping 2 invariants give an error
-                invariant 0 <= index <= omDS.Length
-                invariant forall i :: 0 <= i < index ==> omDS[i] == null || (omDS[i] != null && omDS[i].omValue != x)
-                decreases omDS.Length - index
-            {
-                if(omDS[index] != null && omDS[index].omValue == x) {
-                    break;
-                }
-
-                index := index + 1;
-            }
-        }
-
-        method findIndexUnknownVal(x: int) returns (index: int)
-            ensures -1 <= index < omDS.Length
-            ensures index == -1 || ((exists i :: 0 <= i < omDS.Length && (omDS[i] != null && omDS[i].omValue == x)) && index >= 0)
-        {
-            var indexInner: int := 0;
-            index := -1; // not found is -1
-            while(indexInner < omDS.Length)
-                // Swapping 2 invariants give an error
-                invariant 0 <= indexInner <= omDS.Length
-                invariant forall i :: 0 <= i < indexInner ==> omDS[i] == null || (omDS[i] != null && omDS[i].omValue != x)
-                decreases omDS.Length - indexInner
-            {
-                if(omDS[indexInner] != null && omDS[indexInner].omValue == x) {
-                    index := indexInner;
-                    break;
-                }
-
-                indexInner := indexInner + 1;
-            }
-        }
-
-        // This method of copying values and labels was added due to seq are immutable and arrays are fixed length.
-        // Method params are immutable.
-        method addValBeforeIndex(yIndex: int, x: int, xLabel: int)
-            requires exists i :: 0 <= i < omDS.Length && omDS[i] != null && i == yIndex
-            modifies omDS
-        {
-            var index: int := yIndex;
-
-            var yNode: Node := omDS[index];
-            omDS[index] := new Node(xLabel, x);
-            index := index + 1;
-
-            // Can't assert below. Should be a limitation of Dafny
-            // assert omDS[yIndex].omValue == x;
-
-            while(index < omDS.Length)
-                invariant yIndex+1 <= index <= omDS.Length
-                invariant forall i :: yIndex+1 <= i < index ==> omDS[i] != null
-                decreases omDS.Length - index
-            {
-                var yNodeNext := omDS[index];
-                omDS[index] := yNode;
-                if(yNodeNext == null) {
-                    break;
-                } else {
-                    yNode := yNodeNext;
-                }
-
-                index := index + 1;
-            }
-
-            // Can't assert below. Should be a limitation of Dafny
-            // assert exists i :: 0 <= i < omDS.Length ==> omDS[i] != null && omDS[i].omValue == x;
-        }
-
-        method addBefore(x: int, y: int)
-            // Check y exists in DS
-            requires exists i :: 0 <= i < omDS.Length && omDS[i] != null && omDS[i].omValue == y
-            // Check x doesn't exist in DS
-            requires forall i :: 0 <= i < omDS.Length && omDS[i] != null && omDS[i].omValue != x
+        method addBefore(x: int, yNode: Node)
             // Check x's position is less than y's position
-            modifies omDS
+            ensures exists i,j :: 0 <= i < j < |omDsSeq| && omDsSeq[i].omValue == x && omDsSeq[j].omValue == yNode.omValue
+            ensures yNode.previous != null && x == yNode.previous.omValue
+            modifies yNode, yNode.previous, omDS, omDsSeq
         {
+            var xNode: Node;
 
-            var yIndex: int := findIndex(y);
-            // yIndex = 0 should trigger relabelling. Thus, not covered in initial version.
-            if(yIndex > 0) {
-                var xLabel := (omDS[yIndex - 1].omLabel + omDS[yIndex].omLabel) / 2;
-                addValBeforeIndex(yIndex, x, xLabel);
-            }
+            if(yNode.previous != null) {
 
-            // Can't assert below. Should be a limitation of Dafny
-            // assert exists i :: 0 <= i < omDS.Length ==> omDS[i] != null && y == omDS[i].omValue;
-            // assert exists i :: 0 <= i < omDS.Length && omDS[i] != null && x == omDS[i].omValue;
-        }
+                var previousNode: Node := yNode.previous;
+                var xLabel := (yNode.previous.omLabel + yNode.omLabel) / 2;
+                
+                xNode := new Node(xLabel, x, yNode.index);
 
-        method addValAfterIndex(yIndex: int, x: int, xLabel: int)
-            requires exists i :: 0 <= i < omDS.Length && omDS[i] != null && i == yIndex
-            modifies omDS
-        {
-            var index: int := yIndex + 1;
+                xNode.previous := previousNode;
+                xNode.next := yNode;
+                yNode.previous := xNode;
+                previousNode.next := xNode;
+                
+                // TODO: Later if time is enough
+                // reIndex(omDS);
 
-            // Otherwise needs relabelling or max capacity is reached.
-            if(index < omDS.Length) {
-
-                var yNodeNext: Node? := omDS[index];
-                omDS[index] := new Node(xLabel, x);
-                index := index + 1;
-
-                // Can't assert below. Should be a limitation of Dafny
-                // assert omDS[yIndex+1].omValue == x;
-
-                while(yNodeNext != null && index < omDS.Length)
-                    invariant yIndex+2 <= index <= omDS.Length
-                    invariant forall i :: yIndex+2 <= i < index ==> omDS[i] != null
-                    decreases omDS.Length - index
-                {
-                    var yNodeNextNext := omDS[index];
-                    omDS[index] := yNodeNext;
-                    if(yNodeNextNext == null) {
-                        break;
-                    } else {
-                        yNodeNext := yNodeNextNext;
-                    }
-
-                    index := index + 1;
-                }
-
-                // Can't assert below. Should be a limitation of Dafny
-                // assert exists i :: 0 <= i < omDS.Length ==> omDS[i] != null && omDS[i].omValue == x;
-            }
-        }
-
-        method addAfter(x: int, y: int)
-            // Check y exists in the array
-            requires exists i :: 0 <= i < omDS.Length && omDS[i] != null && y == omDS[i].omValue
-            // Check x doesn't exist in the array
-            requires forall i :: 0 <= i < omDS.Length && omDS[i] != null && x != omDS[i].omValue
-            modifies omDS
-        {
-            var yIndex: int := findIndex(y);
-            // yIndex = 0 should trigger relabelling. Thus, not covered in initial version.
-            var xLabel: int := 0;
-            if(yIndex == omDS.Length-1) {
-                xLabel := (omDS[yIndex].omLabel + (omDS.Length * omDS.Length)) / 2;
             } else {
-                xLabel := (omDS[yIndex].omLabel + omDS[yIndex + 1].omLabel) / 2;
-            }
-            addValAfterIndex(yIndex, x, xLabel);
-        }
+                // Add before value to starting spot should relabel.
+                var xLabel := (0 + yNode.omLabel) / 2;
+                
+                xNode := new Node(xLabel, x, 0);
 
-        method addValAtIndex(yIndex: int, x: int, xLabel: int)
-            requires 0 <= yIndex < omDS.Length
-            modifies omDS
-        {
-            var index: int := yIndex;
+                xNode.next := yNode;
+                yNode.previous := xNode;
 
-            var yNode: Node? := omDS[index];
-            omDS[index] := new Node(xLabel, x);
-            index := index + 1;
-
-            // Can't assert below. Should be a limitation of Dafny
-            // assert omDS[yIndex].omValue == x;
-
-            while(yNode != null && index < omDS.Length)
-                invariant yIndex+1 <= index <= omDS.Length
-                invariant forall i :: yIndex+1 <= i < index ==> omDS[i] != null
-                decreases omDS.Length - index
-            {
-                var yNodeNext := omDS[index];
-                omDS[index] := yNode;
-                if(yNodeNext == null) {
-                    break;
-                } else {
-                    yNode := yNodeNext;
-                }
-
-                index := index + 1;
+                // TODO: Later if time is enough
+                // relabel();
             }
 
-            // Can't assert below. Should be a limitation of Dafny
-            // assert exists i :: 0 <= i < omDS.Length ==> omDS[i] != null && omDS[i].omValue == x;
+            omDsSeq := omDsSeq[..yNode.index] + [xNode] + omDsSeq[yNode.index..];
         }
 
-        method add(x: int)
-            // Check x doesn't exist in DS
-            requires forall i :: 0 <= i < omDS.Length && omDS[i] != null && omDS[i].omValue != x
-            modifies omDS
+        // method reIndex(omDS: Node?)
+        //     modifies omDS
+        // {
+        //     var currentNode: Node? := omDS;
+        //     var index: int := 0;
+
+        //     while(currentNode != null)
+        //         decreases |omDsSeq| - index
+        //     {
+        //         currentNode.index := index;
+        //         index := index + 1;
+        //         currentNode := currentNode.next;
+        //     }
+        // }
+
+        // method relabel()
+        //     modifies omDS
+        // {
+        //     index := 0;
+        //     var newLabel: int, newPos := 0, 0;
+        //     while(index < omDS.Length)
+        //         invariant 0 <= index <= omDS.Length
+        //         decreases omDS.Length - index
+        //         modifies omDS
+        //     {
+        //         if(omDS[index] != null && newPos <= index) {
+        //             omDS[newPos] := new Node(newLabel, omDS[index].omValue);
+
+        //             newLabel := newLabel + currentNumElements;
+        //             newPos := newPos + 1;
+        //         }
+
+        //         index := index + 1;
+        //     }
+        // }
+
+        method addAfter(x: int, yNode: Node)
+            // Check x's position is greater than y's position
+            ensures exists i,j :: 0 <= i < j < |omDsSeq| && omDsSeq[i].omValue == yNode.omValue && omDsSeq[j].omValue == x
+            modifies omDS, omDsSeq, yNode, yNode.next
         {
-            var randomNumber: int := 0;
-            randomNumber := if omDS.Length != 0 then (randomNumberGlobal + randomNumber) % omDS.Length else 0;
-            assert 0 <= randomNumber < omDS.Length;
-            var yIndex: int := randomNumber;
-            var xLabel: int;
-            if(omDS.Length == 0) {
-                xLabel := 1; // Relabelling should be triggered in the next element addition
-            } else if(yIndex == omDS.Length-1) {
-                xLabel := (omDS[yIndex].omLabel + (omDS.Length * omDS.Length)) / 2;
+            var xNode: Node;
+
+            if(yNode.next != null) {
+
+                var nextNode: Node := yNode.next;
+                var xLabel := (yNode.omLabel + yNode.next.omLabel) / 2;
+                
+                xNode := new Node(xLabel, x, yNode.index+1);
+
+                xNode.next := nextNode;
+                xNode.previous := yNode;
+                yNode.next := xNode;
+                nextNode.previous := xNode;
+                
+                // TODO: Later if time is enough
+                // reIndex(omDS);
+
             } else {
-                xLabel := (omDS[yIndex].omLabel + omDS[yIndex + 1].omLabel) / 2;
+                // Add after value to end spot should not relabel.
+                var listSize: int := yNode.index + 1;
+                var xLabel := (yNode.omLabel + (listSize * listSize) - 1) / 2;
+                
+                xNode := new Node(xLabel, x, listSize);
+
+                xNode.previous := yNode;
+                yNode.next := xNode;
             }
-            randomNumber := randomNumber + 1;
+
+            omDsSeq := omDsSeq[..yNode.index+1] + [xNode] + omDsSeq[yNode.index+1..];
+        }
+
+        // method addValAtIndex(yIndex: int, x: int, xLabel: int)
+        //     requires 0 <= yIndex < omDS.Length
+        //     modifies omDS
+        // {
+        //     var index: int := yIndex;
+
+        //     var yNode: Node? := omDS[index];
+        //     omDS[index] := new Node(xLabel, x);
+        //     index := index + 1;
+
+        //     // Can't assert below. Should be a limitation of Dafny
+        //     // assert omDS[yIndex].omValue == x;
+
+        //     while(yNode != null && index < omDS.Length)
+        //         invariant yIndex+1 <= index <= omDS.Length
+        //         invariant forall i :: yIndex+1 <= i < index ==> omDS[i] != null
+        //         decreases omDS.Length - index
+        //     {
+        //         var yNodeNext := omDS[index];
+        //         omDS[index] := yNode;
+        //         if(yNodeNext == null) {
+        //             break;
+        //         } else {
+        //             yNode := yNodeNext;
+        //         }
+
+        //         index := index + 1;
+        //     }
+
+        //     // Can't assert below. Should be a limitation of Dafny
+        //     // assert exists i :: 0 <= i < omDS.Length ==> omDS[i] != null && omDS[i].omValue == x;
+        // }
+
+        // method add(x: int)
+        //     // Check x doesn't exist in DS
+        //     requires forall i :: 0 <= i < omDS.Length && omDS[i] != null && omDS[i].omValue != x
+        //     modifies omDS
+        // {
+        //     var randomNumber: int := 0;
+        //     randomNumber := if omDS.Length != 0 then (randomNumberGlobal + randomNumber) % omDS.Length else 0;
+        //     assert 0 <= randomNumber < omDS.Length;
+        //     var yIndex: int := randomNumber;
+        //     var xLabel: int;
+        //     if(omDS.Length == 0) {
+        //         xLabel := 1; // Relabelling should be triggered in the next element addition
+        //     } else if(yIndex == omDS.Length-1) {
+        //         xLabel := (omDS[yIndex].omLabel + (omDS.Length * omDS.Length)) / 2;
+        //     } else {
+        //         xLabel := (omDS[yIndex].omLabel + omDS[yIndex + 1].omLabel) / 2;
+        //     }
+        //     randomNumber := randomNumber + 1;
             
-            addValAtIndex(yIndex, x, xLabel);
-        }
+        //     addValAtIndex(yIndex, x, xLabel);
+        // }
 
-        method element(x: int) returns (exist: bool)
-            // At some position, if x exists then return true otherwise false
-            ensures exist == false || ((exists i :: 0 <= i < omDS.Length && (omDS[i] != null && omDS[i].omValue == x)) && exist == true)
-        {
-            var index: int := findIndexUnknownVal(x);
-            if(index >= 0) {
-                exist := true;
-            } else {
-                exist := false;
-            }
-        }
+        // method element(x: int) returns (exist: bool)
+        //     // At some position, if x exists then return true otherwise false
+        //     ensures exist == false || ((exists i :: 0 <= i < omDS.Length && (omDS[i] != null && omDS[i].omValue == x)) && exist == true)
+        // {
+        //     var index: int := findIndexUnknownVal(x);
+        //     if(index >= 0) {
+        //         exist := true;
+        //     } else {
+        //         exist := false;
+        //     }
+        // }
 
-        method before(x: int, y: int) returns (isBefore: bool)
-            // Checks x and y are different values
-            requires x != y
-            // Check x exists in DS
-            requires exists i :: 0 <= i < omDS.Length && omDS[i] != null && omDS[i].omValue == x
-            // Check y exists in DS
-            requires exists j :: 0 <= j < omDS.Length && omDS[j] != null && omDS[j].omValue == y
-            // If x's position is less than y's position then return true otherwise false
-            ensures exists i,j :: 0 <= i < j < omDS.Length && ((((omDS[i] != null && omDS[i].omValue == x) && (omDS[j] != null && omDS[j].omValue == y)) && isBefore == true) || isBefore == false)
-        {
-            var xIndex: int := findIndex(x);
-            var yIndex: int := findIndex(y);
+        // method before(x: int, y: int) returns (isBefore: bool)
+        //     // Checks x and y are different values
+        //     requires x != y
+        //     // Check x exists in DS
+        //     requires exists i :: 0 <= i < omDS.Length && omDS[i] != null && omDS[i].omValue == x
+        //     // Check y exists in DS
+        //     requires exists j :: 0 <= j < omDS.Length && omDS[j] != null && omDS[j].omValue == y
+        //     // If x's position is less than y's position then return true otherwise false
+        //     ensures exists i,j :: 0 <= i < j < omDS.Length && ((((omDS[i] != null && omDS[i].omValue == x) && (omDS[j] != null && omDS[j].omValue == y)) && isBefore == true) || isBefore == false)
+        // {
+        //     var xIndex: int := findIndex(x);
+        //     var yIndex: int := findIndex(y);
 
-            if(xIndex < yIndex) {
-                isBefore := true;
-            } else {
-                isBefore := false;
-            }
-        }
+        //     if(xIndex < yIndex) {
+        //         isBefore := true;
+        //     } else {
+        //         isBefore := false;
+        //     }
+        // }
 
-        method append(x: int)
-            // Check x doesn't exist in DS
-            requires forall i :: 0 <= i < omDS.Length && (omDS[i] != null && omDS[i].omValue != x)
-            // If DS size is 1 then x is at the start of DS or DS size is greater than 1 then x is at the end of the DS.
-            ensures ((omDS.Length == 1 && (omDS[0] != null && omDS[0].omValue == x)) || (omDS.Length > 1 && (exists i :: 0 <= i < omDS.Length-1 && ((omDS[i] != null && omDS[i+1] == null) && omDS[i].omValue == x))))
-            modifies omDS
-        {
-            var index: int := 0;
-            while(index < omDS.Length && omDS[index] != null)
-                invariant 0 <= index <= omDS.Length
-                decreases omDS.Length - index
-            {
-                index := index + 1;
-            }
+        // method append(x: int)
+        //     // Check x doesn't exist in DS
+        //     requires forall i :: 0 <= i < omDS.Length && (omDS[i] != null && omDS[i].omValue != x)
+        //     // If DS size is 1 then x is at the start of DS or DS size is greater than 1 then x is at the end of the DS.
+        //     ensures ((omDS.Length == 1 && (omDS[0] != null && omDS[0].omValue == x)) || (omDS.Length > 1 && (exists i :: 0 <= i < omDS.Length-1 && ((omDS[i] != null && omDS[i+1] == null) && omDS[i].omValue == x))))
+        //     modifies omDS
+        // {
+        //     var index: int := 0;
+        //     while(index < omDS.Length && omDS[index] != null)
+        //         invariant 0 <= index <= omDS.Length
+        //         decreases omDS.Length - index
+        //     {
+        //         index := index + 1;
+        //     }
 
-            var numElements: int := index - 1;
-            var appendLabel: int := (numElements * numElements) - 1;
-            omDS[index] := new Node(appendLabel, x);
-        }
+        //     var numElements: int := index - 1;
+        //     var appendLabel: int := (numElements * numElements) - 1;
+        //     omDS[index] := new Node(appendLabel, x);
+        // }
 
-        method prepend(x: int)
-            // At least 1 position should be empty
-            requires exists i :: 0 <= i < omDS.Length && omDS[i] == null
-            // Last element should be null
-            requires omDS.Length > 0 && omDS[omDS.Length-1] == null
-            // Check x doesn't exist in DS
-            requires forall i :: 0 <= i < omDS.Length && omDS[i] != null && omDS[i].omValue != x
-            // Check x is at the start of the DS always
-            ensures omDS.Length > 0 && omDS[0] != null && omDS[0].omValue == x
-            modifies omDS
-        {
-            addValAtIndex(0, x, 0);
+        // method prepend(x: int)
+        //     // At least 1 position should be empty
+        //     requires exists i :: 0 <= i < omDS.Length && omDS[i] == null
+        //     // Last element should be null
+        //     requires omDS.Length > 0 && omDS[omDS.Length-1] == null
+        //     // Check x doesn't exist in DS
+        //     requires forall i :: 0 <= i < omDS.Length && omDS[i] != null && omDS[i].omValue != x
+        //     // Check x is at the start of the DS always
+        //     ensures omDS.Length > 0 && omDS[0] != null && omDS[0].omValue == x
+        //     modifies omDS
+        // {
+        //     addValAtIndex(0, x, 0);
 
-            relabel();
-        }
+        //     relabel();
+        // }
 
-        method relabel()
-            modifies omDS
-        {
-            // Get number of elements in the array
-            var currentNumElements: int := 0;
-            var index: int := 0;
-            while(index < omDS.Length)
-                invariant 0 <= index <= omDS.Length
-                decreases omDS.Length - index
-            {
-                if(omDS[index] != null) {
-                    currentNumElements := currentNumElements + 1;
-                }
+        // method remove(x: int)
+        //     // Check x exists in DS
+        //     requires exists i :: 0 <= i < omDS.Length && omDS[i] != null && omDS[i].omValue == x
+        //     // Check each value is unique
+        //     requires forall i :: 0 <= i < omDS.Length-1 && omDS[i] != null && (forall j :: i < j < omDS.Length && omDS[j] != null && omDS[i].omValue != omDS[j].omValue)
+        //     // Check x doesn't exist in DS
+        //     ensures forall i :: 0 <= i < omDS.Length && ((omDS[i] != null && omDS[i].omValue != x) || omDS[i] == null)
+        //     modifies omDS
+        // {
+        //     var index: int := findIndex(x);
 
-                index := index + 1;
-            }
-
-            // Relabel the elements in the array
-            index := 0;
-            var newLabel: int, newPos := 0, 0;
-            while(index < omDS.Length)
-                invariant 0 <= index <= omDS.Length
-                decreases omDS.Length - index
-                modifies omDS
-            {
-                if(omDS[index] != null && newPos <= index) {
-                    omDS[newPos] := new Node(newLabel, omDS[index].omValue);
-
-                    newLabel := newLabel + currentNumElements;
-                    newPos := newPos + 1;
-                }
-
-                index := index + 1;
-            }
-        }
-
-        method remove(x: int)
-            // Check x exists in DS
-            requires exists i :: 0 <= i < omDS.Length && omDS[i] != null && omDS[i].omValue == x
-            // Check each value is unique
-            requires forall i :: 0 <= i < omDS.Length-1 && omDS[i] != null && (forall j :: i < j < omDS.Length && omDS[j] != null && omDS[i].omValue != omDS[j].omValue)
-            // Check x doesn't exist in DS
-            ensures forall i :: 0 <= i < omDS.Length && ((omDS[i] != null && omDS[i].omValue != x) || omDS[i] == null)
-            modifies omDS
-        {
-            var index: int := findIndex(x);
-
-            omDS[index] := null;
-            // Should be relabled since we have assumed all the elements are in the 
-            // starting half of the array then null
-            // (can be either empty or full array too)
-            relabel();
-        }
+        //     omDS[index] := null;
+        //     // Should be relabled since we have assumed all the elements are in the 
+        //     // starting half of the array then null
+        //     // (can be either empty or full array too)
+        //     relabel();
+        // }
     }
     
 }
